Fix adequacy to use new notation for ewp.

coq-osiris/theories/adequacy/ewp_adequacy.v
@@ -7,7 +7,7 @@ From osiris.adequacy.satisfiable Require Import base_logic_extension satisfiable
 Require Import Coq.Program.Equality.
 
 Definition WPTP `{!osirisGS Σ} (π : thpool) (πp : gmap thread (gname * (outcome2 val exn → iProp Σ))): iProp Σ :=
-  ([∗ map] ι ↦ m; '(γ, φ) ∈ π; πp, saved_pred_own γ DfracDiscarded φ ∗ EWP m @ ⊤ <| (ι, ⊥) |> {{ λ o, □ φ o }}).
+  ([∗ map] ι ↦ m; '(γ, φ) ∈ π; πp, saved_pred_own γ DfracDiscarded φ ∗ EWP[ι] m @ ⊤ <| ⊥ |> {{ λ o, □ φ o }}).
 
 Definition is_final {A E} (m : micro A E) : Prop :=
   match m with
@@ -102,7 +102,7 @@ Qed.
 
 (* [wp_wptp] established the correspondence between [EWP] and [WPTP] over a singleton. *)
 Lemma wp_wptp `{!osirisGS Σ} ι m γ φ :
-  (saved_pred_own γ DfracDiscarded φ ∗ EWP m @ ⊤ <| (ι, ⊥) |> {{ λ o, □ φ o }}) ⊣⊢ WPTP {[ι := m ]} {[ι := (γ, φ)]}.
+  (saved_pred_own γ DfracDiscarded φ ∗ EWP[ι] m @ ⊤ <| ⊥ |> {{ λ o, □ φ o }}) ⊣⊢ WPTP {[ι := m ]} {[ι := (γ, φ)]}.
 Proof.
   unfold WPTP.
   by rewrite big_sepM2_singleton.
@@ -130,7 +130,7 @@ Lemma WPTP_extract_wp `{!osirisGS Σ} π πp ι e :
   WPTP π πp -∗
   ∃ γ φ , ⌜πp !! ι = Some (γ, φ)⌝ ∗
          saved_pred_own γ DfracDiscarded φ ∗
-         EWP e @ ⊤ <| (ι, ⊥) |> {{ λ o, □ φ o }} ∗ WPTP (delete ι π) (delete ι πp).
+         EWP[ι] e @ ⊤ <| ⊥ |> {{ λ o, □ φ o }} ∗ WPTP (delete ι π) (delete ι πp).
 Proof.
   iIntros "%Hlookup Hwps".
   iPoseProof (WPTP_dom with "Hwps") as "%Hdomeq".
@@ -147,7 +147,7 @@ Qed.
 Lemma WPTP_insert_delete `{!osirisGS Σ} ι π1 πp m' γ φ :
   ⌜πp !! ι = Some (γ, φ)⌝ -∗
   WPTP (delete ι π1) (delete ι πp) -∗
-  (saved_pred_own γ DfracDiscarded φ ∗ EWP m' <|(ι, ⊥)|> {{ λ o, □ φ o }}) -∗
+  (saved_pred_own γ DfracDiscarded φ ∗ EWP[ι] m' <|⊥|> {{ λ o, □ φ o }}) -∗
   WPTP (<[ι:=m']> π1) πp.
 Proof.
   iIntros "%Hlookup Hwps Hwp".
@@ -174,9 +174,8 @@ Proof.
   replace πp with (<[ι:=(γ, φ)]>πp) at 2 by apply (insert_id πp ι (γ, φ) Hlookup_p).
   replace π1 with (<[ι:=inject2 o]>π1) at 2 by apply (insert_id π1 ι (inject2 o) Hlookup).
   iFrame.
-  iApply ewp_fupd. iMod "Hwp". iModIntro.
-  iApply ewp_outcome2.
-  iAssumption.
+  iApply ewpi_fupd. iMod "Hwp". iModIntro.
+  by iApply ewpi_outcome2.
 Qed.
 
 (* Isolate a specific postcondition (i.e. terminated thread) in a [WPTP]. *)
@@ -188,7 +187,7 @@ Proof.
   iIntros "%Hlookup Hwps".
   iPoseProof (WPTP_extract_wp $! Hlookup with "Hwps") as "(%γ & %φ & %Hlookup_p & #Hsaved & Hwp & Hwps)".
   iExists γ, φ. iFrame "∗%#".
-  by iApply (ewp_outcome2_inv with "Hwp").
+  by iApply (ewpi_outcome2_inv with "Hwp").
 Qed.
 
 
@@ -229,7 +228,7 @@ Section satisfiability_weakest_pre.
   Context `{!osirisGS Σ}.
 
   Lemma EWP_not_stuck_post {A X} E (e : micro A X) ι σ πp Φ :
-    state_interp (σ, πp) ∗ EWP e @ E <| (ι, ⊥) |> {{ Φ }} ={E}[∅]▷=∗
+    state_interp (σ, πp) ∗ EWP[ι] e @ E <| ⊥ |> {{ Φ }} ={E}[∅]▷=∗
     ⌜not_stuck e σ (dom πp)⌝ ∗ (∀ o, ⌜e = inject2 o⌝ -∗ Φ o).
   Proof.
     iIntros "(Hsi & Hwp)". rewrite /not_stuck.
@@ -303,8 +302,8 @@ Section satisfiability_weakest_pre.
     saved_pred_own γ DfracDiscarded φ -∗
     □ φ o -∗
     state_interp (σ, πp) -∗
-    EWP Stop CJoin ι' k @ E <| (ι, Ψ) |> {{ Φ }} -∗
-    |={E}[∅]▷=> state_interp (σ, πp) ∗ EWP k o @ E <| (ι, Ψ) |> {{ Φ }}.
+    EWP[ι] Stop CJoin ι' k @ E <| Ψ |> {{ Φ }} -∗
+    |={E}[∅]▷=> state_interp (σ, πp) ∗ EWP[ι] k o @ E <| Ψ |> {{ Φ }}.
   Proof.
     iIntros "%Hlookup Hsaved Hφ Hsi Hwp".
     rewrite ewp_unfold /ewp_pre /=. spec_state.
@@ -524,13 +523,13 @@ Section satisfiability_weakest_pre.
     ⌜threadpool_steps k (σ1, {[ι:=e]}) (σ2, π2)⌝ -∗
     (∃ γ, state_interp (σ1, {[ι:=γ]}) ∗
           saved_pred_own γ DfracDiscarded (λ o, ⌜Φ o⌝)%I ∗
-          EWP e @ ⊤ <| (ι, ⊥) |> {{ (λ o, ⌜Φ o⌝)%I }}) ={⊤}[∅]▷=∗^k
+          EWP[ι] e @ ⊤ <| ⊥ |> {{ (λ o, ⌜Φ o⌝)%I }}) ={⊤}[∅]▷=∗^k
     (∀ ι' e, ⌜π2 !! ι' = Some e⌝ ={⊤}[∅]▷=∗
       ⌜not_stuck e σ2 (dom π2)⌝ ∗
       (∀ o, ⌜π2 !! ι = Some (inject2 o)⌝ -∗ |={⊤}=> □ ⌜Φ o⌝)).
   Proof.
     iIntros "%Hsteps (%γ & Hsi & Hsaved & Hwp)".
-    iPoseProof (ewp_mono with "Hwp []") as "Hwp".
+    iPoseProof (ewpi_mono with "Hwp []") as "Hwp".
     { iIntros (o) "%Ho". instantiate (1:=λ o, (□ ⌜Φ o⌝)%I).
       by iModIntro. }
     iCombine "Hsi Hsaved Hwp" as "Hwps".
@@ -573,7 +572,7 @@ Section satisfiability_weakest_pre.
     SAT m F [view ⊤; supply n]
       (∃ γ, state_interp (σ1, {[ι:=γ]}) ∗
        saved_pred_own γ DfracDiscarded (λ o, ⌜Φ o⌝)%I ∗
-       EWP e @ ⊤ <| (ι, ⊥) |> {{ (λ o, ⌜Φ o⌝)%I }}) →
+       EWP[ι] e @ ⊤ <| ⊥ |> {{ (λ o, ⌜Φ o⌝)%I }}) →
     (* and we take a k-step execution to [e'] and some forked of threads *)
     threadpool_steps k (σ1, {[ι := e]}) (σ2, π2) →
     (* then no thread is stuck *)
@@ -628,7 +627,7 @@ Lemma SAT_ewp_adequacy `{invGpreS Σ} (X: Type) (I: X → osirisGS Σ) σ1 σ2 �
     let inv: invGS_gen HasNoLc Σ := osiris_invGS Σ in (* we ensure that all inferences of [invGS] point to this instance *)
     SAT Alloc F [view ⊤; supply n] (state_interp (σ1, ∅) ∗ P x)) →
   (* prove the weakest precondition for all choices of [X] *)
-  (∀ x, let i: osirisGS Σ := I x in P x ⊢ EWP e @ ⊤ <| (ι, ⊥) |> {{ λ o, ⌜Φ o⌝  }}) →
+  (∀ x, let i: osirisGS Σ := I x in P x ⊢ EWP[ι] e @ ⊤ <| ⊥ |> {{ λ o, ⌜Φ o⌝  }}) →
   (* then any k-step execution is safe: *)
   threadpool_steps k (σ1, {[ι := e]}) (σ2, π2) →
   (∀ ι m, π2 !! ι = Some m → not_stuck m σ2 (dom π2)) ∧
@@ -679,7 +678,7 @@ Section adequacy.
 
   Lemma osiris_adequacy Σ `{!osirisGpreS Σ} (e : micro val exn) ι σ1 π2 σ2 k Φ :
     (* If we can show [EWP e1 {{ True }}] with the ghost state provided by [Σ]. *)
-    (∀ `{!osirisGS Σ}, ⊢ EWP e @ ⊤ <|(ι, ⊥)|> {{ λ o, ⌜Φ o⌝ }}) →
+    (∀ `{!osirisGS Σ}, ⊢ EWP[ι] e @ ⊤ <|⊥|> {{ λ o, ⌜Φ o⌝ }}) →
     (* then any k-step execution is safe: *)
     threadpool_steps k (σ1, {[ι := e]}) (σ2, π2) →
     (∀ ι m, π2 !! ι = Some m → not_stuck m σ2 (dom π2)) ∧
@@ -701,7 +700,7 @@ Section adequacy.
   (* Example of an adequacy statement instantiated with a specific set of [gFunctors]. *)
 
   Definition osiris_adequacy_closed (e : micro val exn) ι σ1 π2 σ2 k Φ :
-    (∀ `{!osirisGS osirisΣ}, ⊢ EWP e @ ⊤ <|(ι, ⊥)|> {{ λ o, ⌜Φ o⌝ }}) →
+    (∀ `{!osirisGS osirisΣ}, ⊢ EWP[ι] e @ ⊤ <|⊥|> {{ λ o, ⌜Φ o⌝ }}) →
     threadpool_steps k (σ1, {[ι :=e]}) (σ2, π2) →
     (∀ ι m, π2 !! ι = Some m → not_stuck m σ2 (dom π2)) ∧
     (∀ o, π2 !! ι = Some (inject2 o) → Φ o).
